Proved array foldi

resources/array_foldi/array_foldi_new.ml
@@ -1,0 +1,9 @@
+open Arr
+
+let foldi (t: 'a array) (init: 'b) (f: int -> 'a -> 'b -> 'b) =
+  let (acc: 'b ref) = ref init in
+  array_iteri (fun (i: int) (x: 'a) -> 
+    acc := f i x !acc
+  ) t;
+  let (res: 'b) = !acc in
+  res
