resources/array_foldi/array_foldi_old.ml
@@ -1,0 +1,11 @@
+open Combinators
+
+
+let foldi (t: 'a array) (init: 'b) (f: int -> 'a -> 'b -> 'b) =
+  let (len: int) = Array.length t in 
+  let (res: 'b) =
+    nat_fold_up 0 len
+     (fun (i: int) (acc: 'b) -> 
+       f i t.(i) acc)
+     init in
+  res
