resources/array_foldi/Verify_array_foldi_new.v
@@ -1,0 +1,37 @@
+Set Implicit Arguments.
+From CFML Require Import WPLib Stdlib.
+From TLC Require Import LibListZ.
+
+From Common Require Import Verify_combinators.
+
+From Common Require Import Tactics Utils Solver.
+From Common Require Import Verify_arr.
+
+From ProofsArrayFoldi Require Import Array_foldi_new_ml.
+
+Lemma array_foldi_spec :
+  forall (A : Type) `{EA : Enc A} (B : Type) `{EB: Enc B}
+         (a : array A) (init: B) (f : func)
+         (l : list A)            (fp: int -> A -> B -> B),
+    (forall (i: int) (x: A) (acc: B), 0 <= i < length l ->
+        SPEC_PURE (f i x acc)
+         POST (fun (acc': B) => \[acc' = fp i x acc])) ->
+  SPEC (foldi a init f)
+  PRE (a ~> Array l)
+  POST (fun (b : B) =>
+          \[b = list_foldi l init fp] \* a ~> Array l).
+Proof using (All).
+  xcf.
+  xref acc.
+  xletopaque tmp Htmp.
+  xapp (array_iteri_spec tmp a l
+          (fun (ls: list A) => acc ~~> list_foldi ls init fp)
+       ). {
+    sis_solve_start.
+    subst; rew_list; math.
+    symmetry; erewrite foldi_rcons; auto.
+    f_equal; auto.
+  }
+  xapp.
+  xvals*.
+Qed.
