resources/array_foldi/Verify_array_foldi_old.v
@@ -1,0 +1,40 @@
+Set Implicit Arguments.
+From CFML Require Import WPLib Stdlib.
+From TLC Require Import LibListZ.
+
+From Common Require Import Verify_combinators.
+
+From Common Require Import Tactics Utils Solver.
+From Common Require Import Verify_list.
+
+From ProofsArrayFoldi Require Import Array_foldi_old_ml.
+
+Lemma array_foldi_spec :
+  forall (A : Type) `{EA : Enc A} (B : Type) `{EB: Enc B}
+         (a : array A) (init: B) (f : func)
+         (l : list A)            (fp: int -> A -> B -> B),
+    (forall (i: int) (x: A) (acc: B), 0 <= i < length l ->
+        SPEC_PURE (f i x acc)
+         POST (fun (acc': B) => \[acc' = fp i x acc])) ->
+  SPEC (foldi a init f)
+  PRE (a ~> Array l)
+  POST (fun (b : B) =>
+          \[b = list_foldi l init fp] \* a ~> Array l).
+Proof using (All).
+  xcf.
+  xapp.
+  xletopaque tmp Htmp.
+  xapp (nat_fold_up_spec  0 (length l) tmp init
+          (fun (i: int) (res: B) =>
+             \[res = list_foldi (take i l) init fp] \*
+               a ~> Array l)
+       ). {
+    sis_solve_start.
+    subst; symmetry; erewrite foldi_rcons; auto; f_equal; auto; sis_normalize_length.
+    rewrite (take_pos_last IA); sis_handle_int_index_prove; try math.
+    repeat f_equal; try math.
+  }
+  { math. }
+  { sis_list_solver; unfold list_foldi; auto.  }
+  xvals*. { sis_list_solver; auto. }
+Qed.
