resources/array_foldi/build-rules.sexp
@@ -1,0 +1,65 @@
+
+(rule
+ (target Dummy.v)
+ (deps ../common/Arr_ml.vo
+../common/Combinators_ml.vo
+../common/Lst_ml.vo
+../common/Opt_ml.vo
+../common/Sseq_ml.vo ../common/Solver.vo
+../common/Tactics.vo
+../common/Utils.vo
+../common/Verify_arr.vo
+../common/Verify_combinators.vo
+../common/Verify_list.vo
+../common/Verify_opt.vo
+../common/Verify_sseq.vo
+../common/Verify_vec.vo)
+ (action (run touch Dummy.v)))
+
+
+
+(rule
+     (target array_foldi_new.sisyphus.ml)
+     (deps array_foldi_new.ml)
+     (action (with-stdout-to array_foldi_new.sisyphus.ml
+          (run sed -E "s/\\[@.*\\]//" array_foldi_new.ml))))
+
+(rule
+ (target Array_foldi_new_ml.v)
+ (deps array_foldi_new.sisyphus.ml ../common/Arr_ml.v
+../common/Combinators_ml.v
+../common/Lst_ml.v
+../common/Opt_ml.v
+../common/Sseq_ml.v ../common/arr.ml
+../common/combinators.ml
+../common/lst.ml
+../common/opt.ml
+../common/sseq.ml ../common/arr.cmj
+../common/combinators.cmj
+../common/lst.cmj
+../common/opt.cmj
+../common/sseq.cmj)
+ (action (run cfmlc -I ../common -o ./Array_foldi_new_ml.v array_foldi_new.sisyphus.ml)))
+
+(rule
+     (target array_foldi_old.sisyphus.ml)
+     (deps array_foldi_old.ml)
+     (action (with-stdout-to array_foldi_old.sisyphus.ml
+          (run sed -E "s/\\[@.*\\]//" array_foldi_old.ml))))
+
+(rule
+ (target Array_foldi_old_ml.v)
+ (deps array_foldi_old.sisyphus.ml ../common/Arr_ml.v
+../common/Combinators_ml.v
+../common/Lst_ml.v
+../common/Opt_ml.v
+../common/Sseq_ml.v ../common/arr.ml
+../common/combinators.ml
+../common/lst.ml
+../common/opt.ml
+../common/sseq.ml ../common/arr.cmj
+../common/combinators.cmj
+../common/lst.cmj
+../common/opt.cmj
+../common/sseq.cmj)
+ (action (run cfmlc -I ../common -o ./Array_foldi_old_ml.v array_foldi_old.sisyphus.ml)))
